\Block{3}{herleid}{Herleid $y=\lognl[256](256 x)$ tot de vorm $y=a+b\cdot \lognl[4](x)$}{\begin{enumerate}\item $y=1+\frac{1}{4}\lognl[4](x)$\item $y=4+\frac{1}{1}\lognl[4](x)$\item $y=2+\frac{1}{4}\lognl[4](x)$\item $y=1+\frac{1}{256}\lognl[4](x)$\end{enumerate}}{0}\hfill%
\Block{3}{herleid}{Herleid $y=\lognl[4](64 x)$ tot de vorm $y=a+b\cdot \lognl[2](x)$}{\begin{enumerate}\item $y=3+\frac{1}{2}\lognl[2](x)$\item $y=2+\frac{1}{3}\lognl[2](x)$\item $y=3+\frac{1}{4}\lognl[2](x)$\item $y=4+\frac{1}{2}\lognl[2](x)$\end{enumerate}}{1}\hfill%
\Block{3}{herleid}{Herleid $y=\lognl[4](4 x)$ tot de vorm $y=a+b\cdot \lognl[2](x)$}{\begin{enumerate}\item $y=1+\frac{1}{2}\lognl[2](x)$\item $y=1+\frac{1}{4}\lognl[2](x)$\item $y=2+\frac{1}{2}\lognl[2](x)$\item $y=2+\frac{1}{1}\lognl[2](x)$\end{enumerate}}{2}\hfill%

        \vfill
        \Block{3}{herleid}{Herleid $y=\lognl[8](8 x)$ tot de vorm $y=a+b\cdot \lognl[2](x)$}{\begin{enumerate}\item $y=1+\frac{1}{3}\lognl[2](x)$\item $y=3+\frac{1}{1}\lognl[2](x)$\item $y=2+\frac{1}{3}\lognl[2](x)$\item $y=1+\frac{1}{8}\lognl[2](x)$\end{enumerate}}{3}\hfill%
\Block{3}{herleid}{Herleid $y=\lognl[16](256 x)$ tot de vorm $y=a+b\cdot \lognl[2](x)$}{\begin{enumerate}\item $y=3+\frac{1}{4}\lognl[2](x)$\item $y=2+\frac{1}{16}\lognl[2](x)$\item $y=4+\frac{1}{2}\lognl[2](x)$\item $y=2+\frac{1}{4}\lognl[2](x)$\end{enumerate}}{4}\hfill%
\Block{3}{herleid}{Herleid $y=\lognl[4](64 x)$ tot de vorm $y=a+b\cdot \lognl[2](x)$}{\begin{enumerate}\item $y=2+\frac{1}{3}\lognl[2](x)$\item $y=4+\frac{1}{2}\lognl[2](x)$\item $y=3+\frac{1}{2}\lognl[2](x)$\item $y=3+\frac{1}{4}\lognl[2](x)$\end{enumerate}}{5}\hfill%


\clearpage

\Block{3}{herleid}{Herleid $y=\lognl[4](4 x)$ tot de vorm $y=a+b\cdot \lognl[2](x)$}{\begin{enumerate}\item $y=2+\frac{1}{1}\lognl[2](x)$\item $y=1+\frac{1}{2}\lognl[2](x)$\item $y=2+\frac{1}{2}\lognl[2](x)$\item $y=1+\frac{1}{4}\lognl[2](x)$\end{enumerate}}{6}\hfill%
\Block{3}{herleid}{Herleid $y=\lognl[9](9 x)$ tot de vorm $y=a+b\cdot \lognl[3](x)$}{\begin{enumerate}\item $y=1+\frac{1}{2}\lognl[3](x)$\item $y=2+\frac{1}{2}\lognl[3](x)$\item $y=2+\frac{1}{1}\lognl[3](x)$\item $y=1+\frac{1}{9}\lognl[3](x)$\end{enumerate}}{7}\hfill%
\Block{3}{herleid}{Herleid $y=\lognl[36](36 x)$ tot de vorm $y=a+b\cdot \lognl[6](x)$}{\begin{enumerate}\item $y=1+\frac{1}{2}\lognl[6](x)$\item $y=2+\frac{1}{2}\lognl[6](x)$\item $y=1+\frac{1}{36}\lognl[6](x)$\item $y=2+\frac{1}{1}\lognl[6](x)$\end{enumerate}}{8}\hfill%

        \vfill
        \Block{3}{herleid}{Herleid $y=\lognl[81](81 x)$ tot de vorm $y=a+b\cdot \lognl[3](x)$}{\begin{enumerate}\item $y=1+\frac{1}{81}\lognl[3](x)$\item $y=2+\frac{1}{4}\lognl[3](x)$\item $y=4+\frac{1}{1}\lognl[3](x)$\item $y=1+\frac{1}{4}\lognl[3](x)$\end{enumerate}}{9}\hfill%
\Block{3}{herleid}{Herleid $y=\lognl[36](36 x)$ tot de vorm $y=a+b\cdot \lognl[6](x)$}{\begin{enumerate}\item $y=1+\frac{1}{2}\lognl[6](x)$\item $y=1+\frac{1}{36}\lognl[6](x)$\item $y=2+\frac{1}{2}\lognl[6](x)$\item $y=2+\frac{1}{1}\lognl[6](x)$\end{enumerate}}{10}\hfill%
\Block{3}{herleid}{Herleid $y=\lognl[4](256 x)$ tot de vorm $y=a+b\cdot \lognl[2](x)$}{\begin{enumerate}\item $y=5+\frac{1}{2}\lognl[2](x)$\item $y=4+\frac{1}{4}\lognl[2](x)$\item $y=2+\frac{1}{4}\lognl[2](x)$\item $y=4+\frac{1}{2}\lognl[2](x)$\end{enumerate}}{11}\hfill%


\clearpage

