\Block{3}{omvorm}{Herleid $y=9+\lognl[3] (1\cdot x+2)$}{\begin{enumerate}\item $x=\frac{2}{1}3^{y-9}$\item $x=\frac{3^{1 y-2}}{9}$\item $x=\lognl[3](1 y - 9)-2$\item $x=\frac{3^{y-9}-2}{1}$\end{enumerate}}{0}\hfill%
\Block{3}{omvorm}{Herleid $y=8+\lognl[4] (11\cdot x+11)$}{\begin{enumerate}\item $x=\frac{4^{11 y-11}}{8}$\item $x=\lognl[4](11 y - 8)-11$\item $x=\frac{4^{y-8}-11}{11}$\item $x=\frac{11}{11}4^{y-8}$\end{enumerate}}{1}\hfill%
\Block{3}{omvorm}{Herleid $y=0+\lognl[4] (3\cdot x+0)$}{\begin{enumerate}\item $x=\frac{4^{y-0}-0}{3}$\item $x=\lognl[4](3 y - 0)-0$\item $x=\frac{4^{3 y-0}}{0}$\item $x=\frac{0}{3}4^{y-0}$\end{enumerate}}{2}\hfill%

        \vfill
        \Block{3}{omvorm}{Herleid $y=1+\lognl[3] (14\cdot x+0)$}{\begin{enumerate}\item $x=\frac{3^{y-1}-0}{14}$\item $x=\frac{3^{14 y-0}}{1}$\item $x=\frac{0}{14}3^{y-1}$\item $x=\lognl[3](14 y - 1)-0$\end{enumerate}}{3}\hfill%
\Block{3}{omvorm}{Herleid $y=0+\lognl[2] (6\cdot x+0)$}{\begin{enumerate}\item $x=\frac{2^{y-0}-0}{6}$\item $x=\frac{2^{6 y-0}}{0}$\item $x=\frac{0}{6}2^{y-0}$\item $x=\lognl[2](6 y - 0)-0$\end{enumerate}}{4}\hfill%
\Block{3}{omvorm}{Herleid $y=14+\lognl[4] (9\cdot x+0)$}{\begin{enumerate}\item $x=\frac{0}{9}4^{y-14}$\item $x=\frac{4^{y-14}-0}{9}$\item $x=\frac{4^{9 y-0}}{14}$\item $x=\lognl[4](9 y - 14)-0$\end{enumerate}}{5}\hfill%


\clearpage

