\thispagestyle{empty}% optional: suppress page numbering
    \noindent
\Block{3}{omvorm}{Herleid $y=0+\lognl[2] (7\cdot x+0)$}{\begin{enumerate}\item $x=\frac{2^{7 y-0}}{0}$\item $x=\frac{2^{y-0}-0}{7}$\item $x=\lognl[2](7 y - 0)-0$\item $x=\frac{0}{7}2^{y-0}$\end{enumerate}}{0}\hfill%
\Block{3}{omvorm}{Herleid $y=5+\lognl[2] (4\cdot x+9)$}{\begin{enumerate}\item $x=\frac{2^{4 y-9}}{5}$\item $x=\frac{9}{4}2^{y-5}$\item $x=\frac{2^{y-5}-9}{4}$\item $x=\lognl[2](4 y - 5)-9$\end{enumerate}}{1}\hfill%
\Block{3}{omvorm}{Herleid $y=0+\lognl[2] (8\cdot x+1)$}{\begin{enumerate}\item $x=\frac{2^{8 y-1}}{0}$\item $x=\frac{2^{y-0}-1}{8}$\item $x=\frac{1}{8}2^{y-0}$\item $x=\lognl[2](8 y - 0)-1$\end{enumerate}}{2}\hfill%

        \vfill
        \noindent
        \Block{3}{omvorm}{Herleid $y=0+\lognl[3] (7\cdot x+3)$}{\begin{enumerate}\item $x=\frac{3^{7 y-3}}{0}$\item $x=\frac{3^{y-0}-3}{7}$\item $x=\frac{3}{7}3^{y-0}$\item $x=\lognl[3](7 y - 0)-3$\end{enumerate}}{3}\hfill%
\Block{3}{omvorm}{Herleid $y=0+\lognl[3] (10\cdot x+6)$}{\begin{enumerate}\item $x=\frac{3^{10 y-6}}{0}$\item $x=\frac{3^{y-0}-6}{10}$\item $x=\lognl[3](10 y - 0)-6$\item $x=\frac{6}{10}3^{y-0}$\end{enumerate}}{4}\hfill%
\Block{3}{omvorm}{Herleid $y=7+\lognl[2] (4\cdot x+0)$}{\begin{enumerate}\item $x=\lognl[2](4 y - 7)-0$\item $x=\frac{0}{4}2^{y-7}$\item $x=\frac{2^{y-7}-0}{4}$\item $x=\frac{2^{4 y-0}}{7}$\end{enumerate}}{5}\hfill%


\clearpage

